Core/Node.v
@@ -174,3 +174,37 @@ Definition procInt (st : State) (tr : InternalTransition) (ts : Timestamp) :=
 (* -----------------*)
 (* CASPER FUNCTIONS *)
 (* -----------------*)
+
+Definition processContractCall (st : CasperData) (t : Transaction) : CasperData :=
+  let: validators := casper_validators st in
+  match tx_call t with
+  | DepositCall d =>
+    let: amount := deposit_amount d in
+    let: deposit := (casper_current_dynasty st) \\-> amount in
+    let: validator_index := casper_next_validator_index st in
+    let: validation_addr := deposit_validation_addr d in
+    let: withdrawal_addr := deposit_withdrawal_addr d in
+    let: current_epoch := casper_current_epoch st in
+    let: start_dynasty := (casper_current_dynasty st).+2 in
+    let: end_dynasty := casper_default_end_dynasty in
+    let: validator_data := mkValidatorData validation_addr withdrawal_addr deposit start_dynasty end_dynasty in
+    let: new_validators := validator_index \\-> validator_data \+ validators in
+    mkCasperData
+      (casper_epochs st)
+      new_validators
+      (casper_current_dynasty st)
+      (casper_current_epoch st)
+      (casper_expected_target_hash st)
+      (casper_expected_source_epoch st)
+      (casper_last_justified_epoch st)
+      (casper_last_finalized_epoch st)
+      (casper_dynasty_start_epoch st)
+      (casper_total_curr_dyn_deposits st)
+      (casper_total_prev_dyn_deposits st)
+      (casper_next_validator_index st).+1
+  | VoteCall v => st
+  | LogoutCall l => st
+  | WithdrawCall vi => st
+  | InitializeEpochCall e => st
+  | SlashCall v1 v2 => st
+  end.
